theories/lithium/simpl_instances.v
@@ -210,6 +210,16 @@ Proof. split; destruct b; naive_solver. Qed.
 Global Instance simpl_Z_to_bool_1 (b : bool) : SimplBothRel (=) 1 (Z_of_bool b) (b = true).
 Proof. split; destruct b; naive_solver. Qed.
 
+(* Using a SimplBothRel does not work since [x ≠ y] (i.e., [not (x = y)]) does
+not unify with [?R ?x ?y] (Coq's unification is too limited here). This can be
+seen by applying [simpl_both_rel_inst2], which given the following error:
+[Unable to unify "?Goal1 ?Goal2 ?Goal3" with "0 = Z_of_bool _b_ → False"] *)
+(*Global Instance simpl_Z_to_bool_nonzero b: SimplBothRel (≠) 0 (Z_of_bool b) (b = true).*)
+Global Instance simpl_Z_to_bool_nonzero_1 b : SimplBoth (Z_of_bool b ≠ 0) (b = true).
+Proof. by destruct b. Qed.
+Global Instance simpl_Z_to_bool_nonzero_2 b : SimplBoth (0 ≠ Z_of_bool b) (b = true).
+Proof. by destruct b. Qed.
+
 Global Instance simpl_add_eq_0 n m:
   SimplBothRel (=) (n + m)%nat (0)%nat (n = 0%nat ∧ m = 0%nat).
 Proof. split; naive_solver lia. Qed.
