theories/typing/typing.v
@@ -1,3 +1,3 @@
-From refinedc.typing Require Export programs type int intptr function bytes own struct optional singleton fixpoint automation padded exist immovable constrained union array wand globals tyfold atomic_bool locked tagged_ptr bitfield.
+From refinedc.typing Require Export programs type boolean int intptr function bytes own struct optional singleton fixpoint automation padded exist immovable constrained union array wand globals tyfold atomic_bool locked tagged_ptr bitfield.
 
 Notation "'block{' n }" := (typed_block _ n _ _ _ _) (only printing, format "'block{'  n  }") : bi_scope.
